theories/Typing.v
@@ -4,6 +4,7 @@ From Coq Require Import
 From Hammer Require Import Tactics.
 From LambdaST Require Import
   Context
+  Environment
   Eqb
   FV
   Hole
@@ -48,7 +49,10 @@ Inductive Typed : context -> term -> type -> Prop :=
       Typed Gxs (TmVar x) s
   | TCut : forall G D x e1 e2 s t Gxs GD,
       (* `D` is the context in which we type `e` (as in `let x := e in ...`) *)
-      ~fv G x ->
+      ~fv GD x -> (* <-- TODO: this change (from `G` to `GD`) won't matter theoretically,
+                   * but it avoids problematic cases like `let x := x in x`,
+                   * where technically the second `x` is not shadowed,
+                   * since we carved the first `x` out of the context with its hole *)
       Typed D e1 s ->
       Fill G (CtxHasTy x s) Gxs ->
       Fill G D GD ->
@@ -88,6 +92,111 @@ Proof.
 Qed.
 Hint Resolve typing_fv : core.
 
+Theorem fv_hole_minus : forall GD,
+  WFContext GD ->
+  forall G D,
+  Fill G D GD ->
+  SetEq (fv G) (set_minus (fv GD) (fv D)).
+Proof.
+  intros GD Hw G D Hf. generalize dependent GD. generalize dependent D.
+  induction G; cbn in *; intros.
+  - sinvert Hf. split; tauto.
+  - sinvert Hf. sinvert Hw. eassert (A := IHG _ _ H1 H3). split; intros.
+    2: { repeat destruct H. { right. apply A. split; assumption. } left. assumption. }
+    split. { destruct H. { right. assumption. } apply A in H as [H _]. left. assumption. }
+    intro C. destruct H; [| apply A in H; tauto].
+    assert (H0 := H1). eapply wf_hole_iff in H0 as [Hh [HD Hd]]; [| eassumption].
+    apply fv_fill in H3. apply H4 in H. apply H. apply H3. left. assumption.
+  - sinvert Hf. sinvert Hw. eassert (A := IHG _ _ H2 H3). split; intros.
+    2: { repeat destruct H. { left. assumption. } right. apply A. split; assumption. }
+    split. { destruct H. { left. assumption. } apply A in H as [H _]. right. assumption. }
+    intro C. destruct H; [| apply A in H; tauto].
+    apply fv_fill in H3. apply H4 in H; [destruct H |]. apply H3. left. assumption.
+  - sinvert Hf. sinvert Hw. eassert (A := IHG _ _ H1 H3). split; intros.
+    2: { repeat destruct H. { right. apply A. split; assumption. } left. assumption. }
+    split. { destruct H. { right. assumption. } apply A in H as [H _]. left. assumption. }
+    intro C. destruct H; [| apply A in H; tauto].
+    assert (H0 := H1). eapply wf_hole_iff in H0 as [Hh [HD Hd]]; [| eassumption].
+    apply fv_fill in H3. apply H4 in H. apply H. apply H3. left. assumption.
+  - sinvert Hf. sinvert Hw. eassert (A := IHG _ _ H2 H3). split; intros.
+    2: { repeat destruct H. { left. assumption. } right. apply A. split; assumption. }
+    split. { destruct H. { left. assumption. } apply A in H as [H _]. right. assumption. }
+    intro C. destruct H; [| apply A in H; tauto].
+    apply fv_fill in H3. apply H4 in H; [destruct H |]. apply H3. left. assumption.
+Qed.
+Hint Resolve fv_hole_minus : core.
+
+Theorem typed_deeper : forall GD,
+  WFContext GD ->
+  forall e s,
+  Typed GD e s ->
+  forall G D,
+  Fill G D GD ->
+  (forall x, fv e x -> fv D x) ->
+  Typed D e s.
+Proof.
+  (*
+  intros GD Hw e s Ht G D HD Hf. generalize dependent Hw. generalize dependent G. generalize dependent D.
+  induction Ht; cbn in *; intros.
+  - constructor; [eapply IHHt1 | eapply IHHt2]; try eassumption; intros x Hx; apply Hf; [left | right]; assumption.
+  - econstructor; [assumption | admit | admit | | |]. econstructor; [assumption | eassumption | assumption | eassumption | | assumption].
+  *)
+
+  intros GD Hw e s Ht G D HD Hf. generalize dependent GD. generalize dependent e.
+  generalize dependent s. generalize dependent D. induction G; cbn in *; intros; sinvert HD. { assumption. }
+  - sinvert Hw. eapply IHG; [assumption | | | eassumption]; [assumption |]; clear IHG.
+    remember (CtxComma lhs' g) as ctx eqn:E. generalize dependent G. generalize dependent g.
+    generalize dependent D. generalize dependent lhs'. induction Ht; cbn in *; intros; sinvert E.
+    + sinvert H. constructor; [eapply IHHt1 | eapply IHHt2]; clear IHHt1 IHHt2; try reflexivity; try eassumption;
+      intros x Hx; apply Hf; [left | right]; assumption.
+    + sinvert H8. sinvert H3.
+      * sinvert H2. cbn in H0. cbn in H1. apply Decidable.not_or in H0. apply Decidable.not_or in H1.
+        econstructor; [assumption | | | eassumption | assumption | shelve];
+        intro C; [apply H0 in C as [] | apply H1 in C as []].
+        Unshelve. eassert (A := H4). eapply wf_hole_iff in A as [Hh [_ Hd]]; [| eassumption].
+        eapply IHHt; [| | reflexivity | | |]; clear IHHt. {
+          eapply wf_hole_iff; [eassumption |]. split. { eapply wf_ctx_hole. { apply H4. } eassumption. }
+          split. { constructor; [constructor | constructor |]. split; congruence. } split; sfirstorder. }
+        2: assumption. 2: {
+          intro test. apply fv_fill in H12. split; intros Htest C. {
+            apply H12 in Htest. cbn in Htest. destruct Htest. { destruct H2; subst; tauto. }
+            cbn in *. apply fv_fill in H11. apply H6 in C. apply C. apply H11. right. assumption. }
+          apply fv_fill in H7. apply fv_fill in H11. assert (A := typing_fv _ _ _ Ht). apply H12 in C.
+          destruct C. { cbn in H2. destruct H2; subst; [apply H0 in Htest as [] | apply H1 in Htest as []]. }
+          apply H6 in Htest. apply Htest. apply H11. right. assumption. }
+        (* TODO: if this doesn't work, everything above is still perfect, so cut below this line *)
+        2: apply FillHere. (* <-- TODO: contentious *)
+        intros test Htest. cbn in *. assert (A := typing_fv _ _ _ Ht).
+        apply fv_fill in H7. apply fv_fill in H11. apply fv_fill in H12. Abort.
+(*
+        best time: 100.
+        eapply typing_fv; eassumption.
+        best.
+
+        { Search e. Search lhs'0. best.
+      * clear IHHt.
+
+      ; (econstructor ; [assumption | | | | |]); clear IHHt. admit. admit. admit. admit. admit. admit. admit. admit. eassumption.
+
+    eapply IHG; [| | eassumption |].
+    + intros x Hx. eapply fv_fill; [eassumption |]. left. apply Hf. assumption.
+    + shelve.
+    + eassumption.
+    +
+
+  intros Gmax e s Ht. induction Ht; cbn in *; intros.
+  - constructor; [apply IHHt1 | apply IHHt2]; try assumption;
+    intros; (apply H0; [| assumption]); [left | right]; assumption.
+  - econstructor; [assumption | eassumption | assumption | eassumption | | assumption].
+    assert (A : ctx_lookup Gzst z = Some (TyPar s t)). { apply ctx_lookup_fill; [| eexists]; eassumption. }
+    assert (Hw' := H4). eapply wf_hole_iff in Hw' as [Hh [Hzst Hd]]; [| eassumption].
+    assert (B := H5 _ (or_introl eq_refl) _ A). Search ctx_lookup.
+    apply ctx_lookup_fill in B; [| eapply wf_hole_iff]. admit. clear IHHt H5 H6. ; [| assumption].
+    Search ctx_lookup.
+    apply ctx_lookup_fill.
+Qed.
+*)
+
 Fixpoint typecheck (G : context) (e : term) (s : type) : bool :=
   match e with
     (* T-Eps-R *)
@@ -108,15 +217,35 @@ Fixpoint typecheck (G : context) (e : term) (s : type) : bool :=
       | CtxSemic G' D', TyDot s t => (typecheck G' e1 s && typecheck D' e2 t && ctx_disj G' D')%bool
       | _, _ => false
       end
-    (* T-Let *)
+    (* T-Cut *)
   | TmLet t x e1 e2 =>
       let fve1 := fv_term_li e1 in
+      let GD := G in
       let (G, D) := zoom_in fve1 G in (
-        (negb (lcontains x (fv_hole_li G))) &&
+        (negb (lcontains x (fv_ctx_li GD))) &&
         typecheck D e1 t &&
         typecheck (fill G (CtxHasTy x t)) e2 s)%bool
-  | _ =>
-      (* TODO *) false
+  | TmLetPar x y z e =>
+      match poke G z with
+      | Some (pair (TyPar tx ty) G) =>
+          let fvG := fv_hole_li G in (
+            (negb (eqb x y)) &&
+            (negb (lcontains x fvG)) &&
+            (negb (lcontains y fvG)) &&
+            typecheck (fill G (CtxComma (CtxHasTy x tx) (CtxHasTy y ty))) e s)%bool
+      | _ => false
+      end
+  | TmLetCat t x y z e =>
+      match poke G z with
+      | Some (pair (TyDot tx ty) G) => (
+          eqb ty t &&
+          let fvG := fv_hole_li G in (
+            (negb (eqb x y)) &&
+            (negb (lcontains x fvG)) &&
+            (negb (lcontains y fvG)) &&
+            typecheck (fill G (CtxSemic (CtxHasTy x tx) (CtxHasTy y ty))) e s))%bool
+      | _ => false
+      end
   end.
 
 Theorem typecheck_not_wrong : forall G,
@@ -138,13 +267,31 @@ Proof.
     apply IHe1 in Ht1; [| assumption]. apply IHe2 in Ht2; [| assumption]. constructor; assumption.
   - assert (Hf := zoom_in_full G (fv_term_li e1)). destruct (zoom_in (fv_term_li e1) G) as [G' D'] eqn:E.
     apply Bool.andb_true_iff in H as [H1 H2]. apply Bool.andb_true_iff in H1 as [Hb H1].
-    destruct (reflect_fv_hole G' bind); sinvert Hb.
-    apply IHe1 in H1; [| eapply wf_ctx_plug; eassumption]. apply IHe2 in H2. 2: {
-      eapply wf_hole_iff. { apply reflect_fill. reflexivity. } split. { eapply wf_ctx_hole; eassumption. }
-      split. { constructor. } assert (A := fv_fill _ _ _ Hf). split; congruence. }
-    econstructor; [eassumption | eassumption | | assumption | eassumption]. apply reflect_fill. reflexivity.
-  - discriminate H.
-  - discriminate H.
+    destruct (reflect_fv_ctx G bind); sinvert Hb.
+    assert (A := Hw). apply (wf_hole_iff _ _ _ Hf) in A as [HG' [HD' Hd]].
+    assert (T1 := IHe1 _ HD' _ H1). eassert (Hw' : WFContext (fill G' (CtxHasTy bind t))). {
+      eapply wf_hole_iff. { apply reflect_fill. reflexivity. } split; [assumption |]. split; [constructor |].
+      assert (A := fv_fill _ _ _ Hf). split; [intros H -> | intros -> H]; apply n; apply A; right; assumption. }
+    assert (T2 := IHe2 _ Hw' _ H2). econstructor; [assumption | eassumption | | eassumption | eassumption].
+    apply reflect_fill. reflexivity.
+  - destruct (poke G bound) as [[h z] |] eqn:Ep; [| discriminate H].
+    destruct h; try discriminate H. repeat apply Bool.andb_true_iff in H as [H].
+    destruct (String.eqb_spec lhs rhs); sinvert H.
+    destruct (reflect_fv_hole z lhs); sinvert H2.
+    destruct (reflect_fv_hole z rhs); sinvert H1.
+    assert (Hf := poke_fill _ _ _ _ Ep). econstructor; try eassumption. { apply reflect_fill. reflexivity. }
+    apply IHe; [| assumption]. eapply wf_hole_iff. { apply reflect_fill. reflexivity. }
+    split. { eapply wf_ctx_hole; eassumption. } split. { repeat constructor; congruence. } split; hauto q: on.
+  - destruct (poke G bound) as [[h z] |] eqn:Ep; [| discriminate H]. destruct h; try discriminate H.
+    apply Bool.andb_true_iff in H as [He H]. apply Bool.andb_true_iff in H as [H Ht].
+    apply Bool.andb_true_iff in H as [H Hr]. apply Bool.andb_true_iff in H as [Hn Hl].
+    destruct (String.eqb_spec lhs rhs); sinvert Hn.
+    destruct (reflect_fv_hole z lhs); sinvert Hl.
+    destruct (reflect_fv_hole z rhs); sinvert Hr.
+    destruct (eqb_spec_type h2 t); sinvert He.
+    assert (Hf := poke_fill _ _ _ _ Ep). econstructor; try eassumption. { apply reflect_fill. reflexivity. }
+    apply IHe; [| assumption]. eapply wf_hole_iff. { apply reflect_fill. reflexivity. }
+    split. { eapply wf_ctx_hole; eassumption. } split. { repeat constructor; congruence. } split; hauto q: on.
 Qed.
 
 Theorem typecheck_complete : forall G,
@@ -153,9 +300,58 @@ Theorem typecheck_complete : forall G,
   Typed G e s ->
   typecheck G e s = true.
 Proof.
-  intros G Hw e s Ht. generalize dependent Hw. induction Ht; cbn in *; intros.
-  - rewrite IHHt1; [rewrite IHHt2 |]; [reflexivity | |]; assumption.
-  - Abort.
+  intros G Hw e s Ht. generalize dependent Hw. induction Ht; intros.
+  - cbn. rewrite IHHt1; [rewrite IHHt2 |]; [reflexivity | |]; assumption.
+  - cbn. assert (A := Hw). apply (wf_hole_iff _ _ _ H3) in A as [Hh [Hz Hd]].
+    assert (A : poke Gzst z = Some (pair (TyPar s t) G)); [| rewrite A; clear A]. {
+      apply fill_poke. { apply Hd. reflexivity. } assumption. }
+    repeat (apply Bool.andb_true_iff; split).
+    + apply eqb_neq in H. rewrite H. reflexivity.
+    + destruct (reflect_fv_hole G x); tauto.
+    + destruct (reflect_fv_hole G y); tauto.
+    + assert (E := H2). apply reflect_fill in E. rewrite <- E. clear E.
+      apply IHHt. eapply wf_hole_iff. { eassumption. } split. { assumption. }
+      split. { constructor; [constructor | constructor |]. intro test. split; congruence. }
+      intro test. split; intros Hfv C. destruct C; congruence. destruct Hfv; congruence.
+  - sinvert Hw. cbn. rewrite IHHt1; [| assumption]. rewrite IHHt2; [| assumption].
+    apply (Bool.reflect_iff _ _ (reflect_ctx_disj _ _)) in H4. rewrite H4. reflexivity.
+  - cbn. assert (A := Hw). apply (wf_hole_iff _ _ _ H3) in A as [Hh [Hz Hd]].
+    assert (A : poke Gzst z = Some (pair (TyDot s t) G)); [| rewrite A; clear A]. {
+      apply fill_poke. { apply Hd. reflexivity. } assumption. }
+    repeat (apply Bool.andb_true_iff; split).
+    + destruct (eqb_spec_type t t); [| contradiction n]; reflexivity.
+    + apply eqb_neq in H. rewrite H. reflexivity.
+    + destruct (reflect_fv_hole G x); tauto.
+    + destruct (reflect_fv_hole G y); tauto.
+    + assert (E := H2). apply reflect_fill in E. rewrite <- E. clear E.
+      apply IHHt. eapply wf_hole_iff. { eassumption. } split. { assumption. }
+      split. { constructor; [constructor | constructor |]. intro test. split; congruence. }
+      intro test. split; intros Hfv C. destruct C; congruence. destruct Hfv; congruence.
+  - reflexivity.
+  - reflexivity.
+  - cbn. assert (E : ctx_lookup Gxs x = Some s). { apply ctx_lookup_fill. { assumption. } eexists. eassumption. }
+    rewrite E. destruct (eqb_spec_type s s); [| contradiction n]; reflexivity.
+  - (* Cut/let case. Problem here is that the hole could be in arbitrarily many places and still typecheck.
+     * I believe the trick will be showing that if the hole were any smaller, you couldn't type `e1`,
+     * and if the hole were any larger, you might lose variables in the body.
+     * Let's try induction on the hole in the typing derivation... *)
+    cbn. destruct (zoom_in (fv_term_li e1) GD) as [G0 D0] eqn:E.
+    generalize dependent D. generalize dependent x. generalize dependent e1. generalize dependent e2.
+    generalize dependent s. generalize dependent t. generalize dependent Gxs. generalize dependent GD.
+    generalize dependent G0. generalize dependent D0. induction G; cbn in *; intros.
+    + sinvert H0. sinvert H1. repeat (apply Bool.andb_true_iff; split).
+      * destruct (reflect_fv_ctx GD x); [| reflexivity]. contradiction H.
+      * Abort.
+(*
+    cbn. destruct (zoom_in (fv_term_li e1) GD) as [G0 D0] eqn:E. repeat (apply Bool.andb_true_iff; split).
+    + destruct (reflect_fv_ctx GD x); [| reflexivity]. contradiction H.
+    + admit.
+    + admit.
+  - generalize dependent e. generalize dependent s. generalize dependent Hw. induction H; cbn in *; intros.
+    + apply IHHt. assumption.
+    + sinvert Hw. best.
+Qed.
+*)
 
 Theorem typecheck_correct : forall G,
   WFContext G ->
